Test/separatedclasses/separatedclassesresolutionerrors.dfy
@@ -2,17 +2,23 @@
 // RUN: %diff "%s.expect" "%t"
 
 module SeparatedClasses {
-  predicate {:invariant} WrongInvariant() {
+  predicate {:invariant} WrongInvariant() { // Error: No invariant outside of classes
     true 
   }
   class Class {
-    predicate {:invariant} OneInvariant() {
+    predicate {:invariant} InvariantWithArguments(a: int) { // Error: Invariants can't have arguments
       true
     }
-    predicate {:invariant} SecondInvariant() {
+    predicate {:invariant} InvariantWithTypeParameters<T>() { // Error: Invariants can't have type parameters
       true
     }
-    function {:invariant} NotAnInvariant(): int {
+    predicate {:invariant} OneInvariant() { // OK
+      true
+    }
+    predicate {:invariant} SecondInvariant() { // Error: Duplicate invariant
+      true
+    }
+    function {:invariant} NotAnInvariant(): int { // Error: Functions can't be an invariant
       1
     }
   }
